aneris/examples/transactional_consistency/read_uncommitted/implication_proof/rc_implies_ru.v
@@ -1,0 +1,140 @@
+From iris.algebra Require Import gset auth gmap excl excl_auth csum.
+From iris.base_logic.lib Require Import mono_nat ghost_map.
+From iris.algebra.lib Require Import mono_list.
+From aneris.algebra Require Import monotone.
+From aneris.aneris_lang Require Import network resources proofmode.
+From aneris.lib Require Import gen_heap_light.
+From aneris.aneris_lang.lib Require Import
+     list_proof inject lock_proof.
+From aneris.aneris_lang.lib.serialization
+  Require Import serialization_proof.
+From aneris.examples.reliable_communication.spec
+     Require Import ras.
+From aneris.aneris_lang.program_logic Require Import lightweight_atomic.
+From aneris.examples.transactional_consistency
+     Require Import code_api.
+From aneris.examples.transactional_consistency.read_committed.specs
+  Require Import resources specs.
+From aneris.examples.transactional_consistency.read_uncommitted.specs
+  Require Import resources specs.
+From aneris.examples.transactional_consistency Require Import resource_algebras user_params aux_defs.
+
+Section Implication.
+  Context `{!anerisG Mdl Σ, !KVSG Σ, !User_params, !KVS_transaction_api}.
+
+  Definition OwnAuthSet (γ : gname) (k : Key) (V : Vals) : iProp Σ := own γ (● {[k := V]}).
+  Definition OwnFragSet (γ : gname) (k : Key) (V : Vals) : iProp Σ := own γ (◯ {[k := V]}).
+
+  Lemma ownSetInclusion (γ : gname) (k : Key) (V V' : Vals) : 
+    OwnAuthSet γ k V -∗ 
+    OwnFragSet γ k V' -∗ 
+    OwnAuthSet γ k V ∗ OwnFragSet γ k V' ∗ ⌜V' ⊆ V⌝.
+  Proof.
+    iIntros "Hauth Hfrag".
+    unfold OwnAuthSet, OwnFragSet.
+    iDestruct (own_valid_2 with "Hauth Hfrag") as %[Hord _]%auth_both_valid_discrete.
+    iFrame.
+    iPureIntro.
+    apply (singleton_included k V' V) in Hord as [Hcase1 | Hcase2]; set_solver.
+  Qed.
+
+  Lemma ownSetAdd (γ : gname) (k : Key) (o : option val) (V : Vals) : 
+    OwnAuthSet γ k V ==∗ 
+    OwnAuthSet γ k (V ∪ {[o]}) ∗ OwnFragSet γ k (V ∪ {[o]}).
+  Proof.
+    iIntros "Hauth".
+    unfold OwnAuthSet, OwnFragSet.
+    iMod (own_update _ _ (● (<[k:=(V ∪ {[o]})]> {[k := V]}) ⋅ ◯ {[k := V ∪ {[o]}]}) with "Hauth") as "(Hauth & Hfrag)".
+    - apply auth_update_alloc.
+      apply (insert_alloc_local_update _ _ _ V).
+      + by rewrite lookup_singleton.
+      + by rewrite lookup_empty.
+      + apply gset_local_update.
+        set_solver.
+    - iModIntro.
+      rewrite insert_singleton.
+      iFrame.
+  Qed.
+ 
+  Global Program Instance RU_resources_instance (γ : gname) `(RC : !RC_resources Mdl Σ) : RU_resources Mdl Σ :=
+    {|
+      GlobalInv := RC.(read_committed.specs.resources.GlobalInv);
+      OwnMemKey k V := (∃ (V' : Vals), ⌜V' ⊆ V⌝ ∗ 
+                        RC.(read_committed.specs.resources.OwnMemKey) k V' ∗ OwnAuthSet γ k V)%I;
+      OwnLocalKey k c vo := (∃ (V : Vals), ⌜vo ∈ V⌝ ∗ 
+                            RC.(read_committed.specs.resources.OwnLocalKey) k c vo ∗ OwnFragSet γ k {[vo]})%I;
+      ConnectionState c s sa := RC.(read_committed.specs.resources.ConnectionState) c s sa;
+      IsConnected c sa := RC.(read_committed.specs.resources.IsConnected) c sa;
+      KVS_ru := RC.(read_committed.specs.resources.KVS_rc);
+      KVS_Init := RC.(read_committed.specs.resources.KVS_Init);
+      KVS_ClientCanConnect sa := RC.(read_committed.specs.resources.KVS_ClientCanConnect) sa;
+      Seen k V := OwnFragSet γ k V;
+    |}.
+  Next Obligation.
+    iIntros (γ RC k cst v) "[%V (%Hsub & Hkey & Hfrag)]". 
+    iDestruct (RC.(read_committed.specs.resources.OwnLocalKey_serializable) with "Hkey") as "(Hkey & Hser)".
+    iFrame.
+    by iExists V.
+  Qed.
+  Next Obligation.
+    iIntros (γ RC E k V V' Hsub) "#Hinv (Hfrag & [%V'' (Hsub' & Hkey & Hauth)])".
+    iDestruct (ownSetInclusion with "Hauth Hfrag") as "(Hauth' & Hfrag' & Hsub'')".
+    iModIntro.
+    iFrame.
+    iExists V''.
+    iFrame.
+  Qed.
+
+  Theorem implication_rc_ru : 
+    RC_init → RU_init.
+  Proof.
+    intro RC_init.
+    destruct RC_init.
+    split.
+    iIntros (E cli Hsub).
+    iMod (RC_init_module E cli Hsub) as 
+      "[%Hres (Hrc_keys & Hrc_kvs_init & Hrc_inv & Hrc_conn & Hrc_init_kvs
+       & Hrc_init_cli & %Hrc_read & %Hrc_write & %Hrc_start & %Hrc_com)]".
+    iMod (own_alloc (● (∅ : gmapUR Key (gsetUR (option val))))) as (γ) "Halgebra". 
+    {
+      by apply auth_auth_valid.
+    }
+    iExists (RU_resources_instance γ Hres).
+    iModIntro.
+    simpl.
+    iSplitL "Hrc_keys Halgebra".
+    {
+      admit.
+    }
+    iSplitL "Hrc_kvs_init"; first done.
+    iSplitL "Hrc_inv"; first done.
+    iSplitL "Hrc_conn"; first done.
+    iSplitL "Hrc_init_kvs"; first done.
+    iSplitL "Hrc_init_cli"; first done.
+    iSplitL.
+    {
+      unfold read_spec.
+      iPureIntro.
+      iIntros (c sa E' k Hser) "Hsub' Hk_in Hconn".
+      unfold read_committed.specs.specs.read_spec in Hrc_read.
+      iDestruct (Hrc_read c sa E' k Hser with "Hsub' Hk_in Hconn") as "Hrc_read".
+      iIntros (Φ).
+      iDestruct ("Hrc_read" $! Φ) as "#Hrc_read".
+      iModIntro.
+      simpl.
+      admit.
+    }
+    iSplitL.
+    {
+      unfold read_spec.
+      admit.
+    }
+    iSplitL.
+    {
+      unfold read_spec.
+      admit.
+    }
+    admit.
+  Admitted.
+
+End Implication.
