aneris/examples/transactional_consistency/resource_algebras.v
@@ -7,12 +7,10 @@ From aneris.aneris_lang Require Import lang resources.
 From aneris.aneris_lang.lib Require Import lock_proof.
 From aneris.examples.transactional_consistency.snapshot_isolation.specs Require Import
   time events.
-From aneris.examples.transactional_consistency Require Import user_params.
-
+From aneris.examples.transactional_consistency Require Import aux_defs user_params.
 Import gen_heap_light.
 Import lock_proof.
-
-Canonical Structure ip_addressO := leibnizO ip_address.
+From aneris.examples.reliable_communication.spec Require Import ras.
 
 Class IDBG Σ :=
   {
@@ -39,4 +37,31 @@ Class IDBG Σ :=
 
     (** Lock *)
     IDBG_lockG :> lockG Σ;
+
+    (** Implication Encodings *)
+    IDBG_Encoding :> inG Σ (authR (gmapUR Key (gsetUR (option val))));
   }.
+
+Notation KVSG Σ := (IDBG Σ).
+ 
+Definition KVSΣ : gFunctors :=
+  #[
+      ghost_mapΣ Key (list write_eventO);
+      ghost_mapΣ Key (option val * bool);
+      GFunctor (authR (gmapUR Key (max_prefix_listR write_eventO)));
+      GFunctor ((authR (gen_heapUR Key val)));
+      GFunctor (authR (gmapUR nat (agreeR (gmapUR Key (max_prefix_listR write_eventO)))));
+      GFunctor
+        (authR (gmapUR socket_address (agreeR (leibnizO gname))));
+      GFunctor ((csumR
+                   (exclR unitR)
+                   (agreeR ((gnameO * gnameO * gnameO * gnameO * gnameO) : Type))));
+     GFunctor (exclR unitO);
+     GFunctor (authUR (gsetUR nat));
+     GFunctor (authR (gmapUR Key (gsetUR (option val))));
+     mono_natΣ;
+     ras.SpecChanΣ;
+     lockΣ].
+
+Instance subG_KVSΣ {Σ} : subG KVSΣ Σ → KVSG Σ.
+Proof. econstructor; solve_inG. Qed.
