aneris/examples/transactional_consistency/snapshot_isolation/examples/function_call/function_call_proof.v
@@ -8,7 +8,7 @@ From aneris.aneris_lang.program_logic Require Import
      aneris_weakestpre aneris_adequacy aneris_lifting.
 From iris.base_logic.lib Require Import invariants.
 From aneris.examples.transactional_consistency.snapshot_isolation.specs Require Import
-  time events aux_defs resource_algebras resources specs.
+  time events aux_defs resources specs.
 From aneris.examples.transactional_consistency.snapshot_isolation.examples.function_call
       Require Import function_call_code.
 Import ser_inj.
@@ -17,7 +17,7 @@ From aneris.examples.transactional_consistency.snapshot_isolation.instantiation 
      instantiation_of_init.
 From aneris.examples.transactional_consistency.snapshot_isolation.util Require Import util_proof.
 From aneris.examples.transactional_consistency.snapshot_isolation Require Import snapshot_isolation_code.
-From aneris.examples.transactional_consistency Require Import user_params.
+From aneris.examples.transactional_consistency Require Import resource_algebras user_params.
 
 Definition server_addr := SocketAddressInet "0.0.0.0" 80.
 Definition client1_addr := SocketAddressInet "0.0.0.1" 80.
