aneris/examples/transactional_consistency/snapshot_isolation/util/util_proof.v
@@ -1,12 +1,10 @@
 From aneris.aneris_lang Require Import tactics adequacy proofmode.
 From aneris.examples.transactional_consistency.snapshot_isolation.specs
-  Require Import time events aux_defs resource_algebras
-  resources specs.
+  Require Import time events aux_defs resources specs.
 From aneris.examples.transactional_consistency Require Import user_params.
 From aneris.examples.transactional_consistency.snapshot_isolation.instantiation
   Require Import snapshot_isolation_api_implementation.
-From aneris.examples.transactional_consistency Require Import util_code.
-
+From aneris.examples.transactional_consistency Require Import resource_algebras util_code.
 From aneris.aneris_lang.program_logic Require Import lightweight_atomic.
 From iris.algebra Require Import gmap.
 From iris.algebra Require Import excl.
